WebAssembly/Wasm_Interpreter_Printing.thy
@@ -2,40 +2,26 @@ theory Wasm_Interpreter_Printing imports "Wasm_Interpreter_Properties" begin
 
 definition "run = run_v (2^63) 300"
 
-code_printing
-  constant host_apply_impl \<rightharpoonup> (OCaml) "ImplWrapper.host'_apply'_impl"
+(* host *)
+
+axiomatization
+  Abs_host :: "((s \<times> v list) \<Rightarrow> (s \<times> v list) option) \<Rightarrow> host" and
+  Rep_host :: "host \<Rightarrow> ((s \<times> v list) \<Rightarrow> (s \<times> v list) option)"
+where
+  host_is[code abstype]:
+    "Abs_host (Rep_host h) = h"
+and
+  host_apply_impl_def[code] :
+    "host_apply_impl s tf h vs = ((Rep_host h) (s,vs))"
 
 (* memory *)
 
 code_printing
-  type_constructor byte \<rightharpoonup> (OCaml) "ImplWrapperTypes.byte"
+  type_constructor byte \<rightharpoonup> (OCaml) "ImplWrapper.byte"
 
 code_printing
-  constant msb_byte \<rightharpoonup> (OCaml) "ImplWrapperTypes.msb'_byte"
-| constant zero_byte \<rightharpoonup> (OCaml) "ImplWrapperTypes.zero'_byte"
-| constant negone_byte \<rightharpoonup> (OCaml) "ImplWrapperTypes.negone'_byte"
-
-(*
-declare Rep_bytes_inverse[code abstype]
-declare Rep_mem_inverse[code abstype]
-
-code_printing
-  type_constructor bytes \<rightharpoonup> (OCaml) "Int64.t"
-| type_constructor mem \<rightharpoonup> (OCaml) "ImplWrapperTypes.memory"
-
-code_printing
-  constant mem_size \<rightharpoonup> (OCaml) "ImplWrapper.size"
-(* | constant mem_grow \<rightharpoonup> (OCaml) "ImplWrapper.grow" *)
-| constant load \<rightharpoonup> (OCaml) "ImplWrapper.load"
-| constant store \<rightharpoonup> (OCaml) "ImplWrapper.store"
-| constant load_packed \<rightharpoonup> (OCaml) "ImplWrapper.load'_packed"
-| constant store_packed \<rightharpoonup> (OCaml) "ImplWrapper.store'_packed"
-
-declare mem_size_def[code del]
-declare store_def[code del]
-declare load_def[code del]
-declare store_packed_def[code del]
-declare load_packed_def[code del]
-*)
+  constant msb_byte \<rightharpoonup> (OCaml) "ImplWrapper.msb'_byte"
+| constant zero_byte \<rightharpoonup> (OCaml) "ImplWrapper.zero'_byte"
+| constant negone_byte \<rightharpoonup> (OCaml) "ImplWrapper.negone'_byte"
 
 end
